WIP: Initialization of size_classes

src/Main.fst
@@ -2,27 +2,167 @@ module Main
 
 module U8 = FStar.UInt8
 module U32 = FStar.UInt32
+module U64 = FStar.UInt64
+module US = FStar.SizeT
 
 open SizeClass
 open Steel.Effect.Atomic
 open Steel.Effect
 open Steel.Array
+module A = Steel.Array
+module AR = Steel.ArrayRef
+module R = Steel.Reference
 module L = Steel.SpinLock
+module SL = BlobList
+
+noeq
+type size_class =
+  { data : size_class_struct;
+    lock : L.lock (size_class_vprop data) }
+
+assume val mmap_u8 (len: US.t)
+  : Steel (array U8.t)
+    emp
+    (fun a -> A.varray a)
+    (fun _ -> True)
+    (fun _ a h1 ->
+      A.length a == US.v len /\
+      A.is_full_array a /\
+      A.asel a h1 == Seq.create (US.v len) U8.zero
+    )
+assume val mmap_u64 (len: US.t)
+  : Steel (array U64.t)
+    emp
+    (fun a -> A.varray a)
+    (fun _ -> True)
+    (fun _ a h1 ->
+      A.length a == US.v len /\
+      A.is_full_array a /\
+      A.asel a h1 == Seq.create (US.v len) U64.zero
+    )
+
+assume val mmap_blob (len: US.t)
+  : Steel (array SL.cell)
+     emp
+    (fun a -> A.varray a)
+    (fun _ -> True)
+    (fun _ a h1 ->
+      A.length a == US.v len /\
+      A.is_full_array a
+    )
+
+assume val mmap_ptr_u32 (_:unit)
+  : SteelT (R.ref U32.t)
+    emp
+    (fun r -> R.vptr r)
+
+assume val mmap_ptr_slt (_:unit)
+  : SteelT (R.ref SL.t)
+    emp
+    (fun r -> R.vptr r)
+
+//TODO: move to utils
+let u32_to_sz = Slabs.u32_to_sz
+
+#restart-solver
+#push-options "--z3rlimit 100 --compat_pre_typed_indexed_effects"
+let init (sc:U32.t)
+  : SteelT size_class_struct
+  emp
+  (fun scs -> size_class_vprop scs)
+
+  =
+  let open Utils2 in
+  assume (US.fits_u32);
+  let v : v:U32.t{U32.v v <= U32.v metadata_max == true}
+    = 0ul in
+  let slab_region = mmap_u8 (u32_to_sz (U32.mul metadata_max page_size)) in
+  let md_bm_region = mmap_u64 (u32_to_sz (U32.mul metadata_max 4ul)) in
+  let md_region = mmap_blob (u32_to_sz metadata_max) in
+  A.ghost_split slab_region 0sz;
+  A.ghost_split md_bm_region 0sz;
+  A.ghost_split md_region 0sz;
+  drop (A.varray (A.split_l slab_region 0sz));
+  drop (A.varray (A.split_l md_bm_region 0sz));
+  drop (A.varray (A.split_l md_region 0sz));
+  change_equal_slprop
+    (A.varray (A.split_r slab_region 0sz))
+    (A.varray (A.split_r slab_region (u32_to_sz (U32.mul v page_size))));
+  change_equal_slprop
+    (A.varray (A.split_r md_bm_region 0sz))
+    (A.varray (A.split_r md_bm_region (u32_to_sz (U32.mul v 4ul))));
+  change_equal_slprop
+    (A.varray (A.split_r md_region 0sz))
+    (A.varray (A.split_r md_region (u32_to_sz v)));
+  intro_vrefine
+    (A.varray (A.split_r slab_region (u32_to_sz (U32.mul v page_size)))) zf_u8;
+  intro_vrefine
+    (A.varray (A.split_r md_bm_region (u32_to_sz (U32.mul v 4ul)))) zf_u64;
+  change_slprop_rel
+    ((A.varray (A.split_r slab_region (u32_to_sz (U32.mul v page_size)))
+      `vrefine` zf_u8) `star`
+    (A.varray (A.split_r md_bm_region (u32_to_sz (U32.mul v 4ul)))
+      `vrefine` zf_u64) `star`
+    A.varray (A.split_r md_region (u32_to_sz v)))
+    (Slabs.vp_aux slab_region md_bm_region md_region v)
+    (fun x y -> x == y)
+    (fun _ -> admit ());
+  let md_count = mmap_ptr_u32 () in
+  R.write md_count v;
+  SteelVRefineDep.intro_vrefinedep
+    (R.vptr md_count)
+    (fun x -> U32.v x <= U32.v metadata_max == true)
+    (Slabs.vp_aux slab_region md_bm_region md_region)
+    (Slabs.vp_aux slab_region md_bm_region md_region v);
+
+  let ptr_partial = mmap_ptr_slt () in
+  let ptr_empty = mmap_ptr_slt () in
+  let ptr_full = mmap_ptr_slt () in
+
+  R.write ptr_partial SL.null_t;
+  R.write ptr_empty SL.null_t;
+  R.write ptr_full SL.null_t;
+
+  SL.intro_llist_nil (Slabs.p_partial 16ul);
+  SL.intro_llist_nil (Slabs.p_empty 16ul);
+  SL.intro_llist_nil (Slabs.p_full 16ul);
+
+  SL.pack_ind (Slabs.p_partial 16ul) ptr_partial SL.null_t;
+  SL.pack_ind (Slabs.p_empty 16ul) ptr_empty SL.null_t;
+  SL.pack_ind (Slabs.p_full 16ul) ptr_full SL.null_t;
+
+
+  let scs = {
+    size = 16ul;
+    partial_slabs = ptr_partial;
+    empty_slabs = ptr_empty;
+    full_slabs = ptr_full;
+    slab_region = slab_region;
+    md_bm_region = md_bm_region;
+    md_region = md_region;
+    md_count = md_count;
+  } in
+
+  change_equal_slprop
+   (SL.ind_llist (Slabs.p_partial 16ul) ptr_partial `star`
+    SL.ind_llist (Slabs.p_empty 16ul) ptr_empty `star`
+    SL.ind_llist (Slabs.p_full 16ul) ptr_full `star`
+  SteelVRefineDep.vrefinedep
+    (R.vptr md_count)
+    //TODO: hideous coercion
+    (fun x -> U32.v x <= U32.v metadata_max == true)
+    (Slabs.vp_aux slab_region md_bm_region md_region))
+  (size_class_vprop scs);
+
+  return scs
+
 
 assume
-val size_class16 : size_class_struct
+val size_class16 : size_class
 assume
-val size_class32 : size_class_struct
+val size_class32 : size_class
 assume
-val size_class64 : size_class_struct
-
-assume
-val size_class16_lock : L.lock (size_class_vprop size_class16)
-assume
-val size_class32_lock : L.lock (size_class_vprop size_class32)
-assume
-val size_class64_lock : L.lock (size_class_vprop size_class64)
-
+val size_class64 : size_class
 
 
 let null_or_varray (#a:Type) (r:array a) : vprop = if is_null r then emp else varray r
@@ -59,24 +199,24 @@ let slab_malloc bytes =
     return_null ()
   else begin
     if bytes `U32.lte` 16ul then begin
-      L.acquire size_class16_lock;
-      let ptr = allocate_size_class size_class16 in
-      L.release size_class16_lock;
+      L.acquire size_class16.lock;
+      let ptr = allocate_size_class size_class16.data in
+      L.release size_class16.lock;
       return ptr
     end
     else
     if bytes `U32.lte` 32ul then begin
-      L.acquire size_class32_lock;
-      let ptr = allocate_size_class size_class32 in
-      L.release size_class32_lock;
+      L.acquire size_class32.lock;
+      let ptr = allocate_size_class size_class32.data in
+      L.release size_class32.lock;
       return ptr
 
     end
     else
     if bytes `U32.lte` 64ul then begin
-      L.acquire size_class64_lock;
-      let ptr = allocate_size_class size_class64 in
-      L.release size_class64_lock;
+      L.acquire size_class64.lock;
+      let ptr = allocate_size_class size_class64.data in
+      L.release size_class64.lock;
       return ptr
     end
     else return_null ()
